src/drf/PromiseConsistent.v
@@ -335,3 +335,68 @@ Proof.
 Grab Existential Variables. exact true.
 Qed.
 
+Lemma promise_consistent_th_small_step_forward
+      withprm tid e c1 c2
+      (STEP: small_step withprm tid e c1 c2)
+      (PRCONS: forall tid0, promise_consistent_th tid0 c1)
+      (PRCONS2: promise_consistent_th tid c2)
+      (WF: Configuration.wf c1):
+  forall tid0, promise_consistent_th tid0 c2.
+Proof.
+  i. s. destruct (Ident.eq_dec tid0 tid) eqn: EQ.
+  - subst. eauto.
+  - ii. exploit small_step_find; eauto.
+    s; intro X. rewrite <-X in THREAD. 
+    eapply (PRCONS tid0); eauto.  
+Qed.
+
+Lemma rtc_promise_consistent_th_small_step_forward
+      withprm tid c1 c2
+      (STEP: rtc (small_step_evt withprm tid) c1 c2)
+      (PRCONS: forall tid0, promise_consistent_th tid0 c1)
+      (PRCONS2: promise_consistent_th tid c2)
+      (WF: Configuration.wf c1):
+  forall tid0, promise_consistent_th tid0 c2.
+Proof.
+  apply Operators_Properties.clos_rt_rt1n_iff,
+        Operators_Properties.clos_rt_rtn1_iff in STEP.
+  ginduction STEP; eauto.
+  apply Operators_Properties.clos_rt_rtn1_iff,
+        Operators_Properties.clos_rt_rt1n_iff in STEP.
+  i. inv H. hexploit promise_consistent_th_small_step_forward; eauto; cycle 1.
+  { eapply rtc_small_step_future; eauto.
+    eapply rtc_implies, STEP. eauto. }
+  i. hexploit IHSTEP; eauto.
+  eapply promise_consistent_th_small_step; eauto.
+  eapply rtc_small_step_future; eauto.
+  eapply rtc_implies, STEP. eauto.
+Qed.
+
+Lemma promise_consistent_th_small_step_backward
+      withprm tid e c1 c2
+      (STEP: small_step withprm tid e c1 c2)
+      (PRCONS: forall tid0, promise_consistent_th tid0 c2)
+      (WF: Configuration.wf c1):
+  forall tid0, promise_consistent_th tid0 c1.
+Proof.
+  i. s. destruct (Ident.eq_dec tid0 tid) eqn: EQ.
+  - subst. hexploit promise_consistent_th_small_step; eauto.
+  - ii. exploit small_step_find; eauto.
+    s; intro X. rewrite X in THREAD. 
+    eapply (PRCONS tid0); eauto.  
+Qed.
+
+Lemma rtc_promise_consistent_th_small_step_backward
+      withprm tid c1 c2
+      (STEP: rtc (small_step_evt withprm tid) c1 c2)
+      (PRCONS: forall tid0, promise_consistent_th tid0 c2)
+      (WF: Configuration.wf c1):
+  forall tid0, promise_consistent_th tid0 c1.
+Proof.
+  ginduction STEP; eauto.
+  i. inv H. 
+  i. hexploit promise_consistent_th_small_step_backward; eauto.
+  i. hexploit IHSTEP; eauto.
+  eapply small_step_future; eauto.
+Qed.
+
