src/lib/Basic.v
@@ -172,6 +172,12 @@ Qed.
 Definition option_app {A} (a b: option A) : option A :=
   if a then a else b.
 
+Definition option_rel {A B} (P: A -> B -> Prop) : option A -> option B -> Prop :=
+  fun a b => match a, b with 
+             | Some x, Some y => P x y 
+             | None, None => True 
+             | _, _ => False end.
+
 Lemma strengthen
       (A B: Prop)
       (H: A /\ (A -> B)):
