src/opt/ProgressStep.v
@@ -1,0 +1,68 @@
+Require Import Basics.
+Require Import Bool.
+Require Import List.
+
+Require Import sflib.
+Require Import paco.
+Require Import respectful5.
+
+Require Import Basic.
+Require Import DenseOrder.
+Require Import Event.
+Require Import Language.
+Require Import Time.
+Require Import View.
+Require Import Cell.
+Require Import Memory.
+Require Import MemoryFacts.
+Require Import TView.
+Require Import Thread.
+Require Import Configuration.
+Require Import Progress.
+
+Require Import Syntax.
+Require Import Semantics.
+
+Set Implicit Arguments.
+
+Lemma progress_program_step
+      rs1 i1 s1 lc1 sc1 mem1
+      (WF1: Local.wf lc1 mem1)
+      (MEM1: Memory.closed mem1)
+      (SC1: Memory.closed_timemap sc1 mem1)
+      (PROMISES1: lc1.(Local.promises) = Memory.bot):
+  exists e th2, <<STEP: Thread.program_step e (Thread.mk lang (State.mk rs1 (i1::s1)) lc1 sc1 mem1) th2>>.
+Proof.
+  destruct i1.
+  - destruct i.
+    + esplits. econs; [|econs 1]; eauto. econs. econs.
+    + esplits. econs; [|econs 1]; eauto. econs. econs.
+    + hexploit progress_read_step; eauto. i. des.
+      esplits. econs; [|econs 2]; eauto. econs. econs.
+    + hexploit progress_write_step; eauto.
+      { apply Time.incr_spec. }
+      { econs 2. }
+      { econs. }
+      { i. rewrite PROMISES1. apply Memory.bot_nonsynch_loc. }
+      i. des. esplits. econs; [|econs 3]; eauto. econs. econs.
+    + hexploit progress_read_step; eauto. i. des.
+      exploit Local.read_step_future; eauto. i. des.
+      destruct (RegFile.eval_rmw rs1 rmw val) as [? []] eqn: EQ.
+      * hexploit progress_write_step; eauto.
+        { apply Time.incr_spec. }
+        { i. inv H. s. rewrite PROMISES1. apply Memory.bot_nonsynch_loc. }
+        i. des. esplits. econs; [|econs 4]; eauto. econs. econs. rewrite EQ. eauto.
+      * esplits. econs; [|econs 2]; eauto. econs. econs. rewrite EQ; eauto.
+    + hexploit progress_fence_step; eauto.
+      { i. rewrite PROMISES1. apply Memory.bot_nonsynch. }
+      i. des.
+      esplits. econs; [|econs 5]; eauto. econs. econs.
+    + hexploit progress_fence_step; eauto.
+      { i. rewrite PROMISES1. apply Memory.bot_nonsynch. }
+      i. des.
+      esplits. econs; [|econs 6]; eauto. econs. econs.
+  - esplits. econs; [|econs 1]; eauto. econs.
+  - esplits. econs; [|econs 1]; eauto. econs.
+Grab Existential Variables.
+  { auto. }
+Qed.
